add perservatino

new_proof/BasicTyping.v
@@ -60,22 +60,22 @@ Reserved Notation "Γ '⊢t' t '⋮t' T" (at level 40).
 Reserved Notation "Γ '⊢t' t '⋮v' T" (at level 40).
 
 Inductive tm_has_type : context -> tm -> ty -> Prop :=
-| T_Err : forall Γ T, Γ ⊢t terr ⋮t T
+| T_Err : forall Γ T, ok Γ -> Γ ⊢t terr ⋮t T
 | T_Value : forall Γ v T, Γ ⊢t v ⋮v T -> Γ ⊢t v ⋮t T
 | T_Lete : forall Γ e1 e2 T1 T2 (L: aset),
     Γ ⊢t e1 ⋮t T1 ->
-    (forall (x: atom), x ∉ L -> (Γ ++ [(x, T1)]) ⊢t e2 ⋮t T2) ->
+    (forall (x: atom), x ∉ L -> (Γ ++ [(x, T1)]) ⊢t e2 ^t^ x ⋮t T2) ->
     Γ ⊢t (tlete e1 e2) ⋮t T2
 | T_LetOp : forall Γ (op: biop) v1 v2 e (T1 T2 Tx: base_ty) T (L: aset),
     Γ ⊢t v1 ⋮v T1 ->
     Γ ⊢t v2 ⋮v T2 ->
-    ty_of_op op = T1 ⤍ T2 ⤍ Tx ->
-    (forall (x: atom), x ∉ L -> (Γ ++ [(x, TBase Tx)]) ⊢t e ⋮t T) ->
+    Γ ⊢t op ⋮v T1 ⤍ T2 ⤍ Tx ->
+    (forall (x: atom), x ∉ L -> (Γ ++ [(x, TBase Tx)]) ⊢t e ^t^ x ⋮t T) ->
     Γ ⊢t tletbiop op v1 v2 e ⋮t T
 | T_LetApp : forall Γ v1 v2 e (T1 Tx: base_ty) T (L: aset),
-    Γ ⊢t v1 ⋮v T1 ->
-    Γ ⊢t v2 ⋮v T1 ⤍ Tx ->
-    (forall (x: atom), x ∉ L -> (Γ ++ [(x, TBase Tx)]) ⊢t e ⋮t T) ->
+    Γ ⊢t v1 ⋮v T1 ⤍ Tx ->
+    Γ ⊢t v2 ⋮v T1 ->
+    (forall (x: atom), x ∉ L -> (Γ ++ [(x, TBase Tx)]) ⊢t e ^t^ x ⋮t T) ->
     Γ ⊢t tletapp v1 v2 e ⋮t T
 | T_Matchb: forall Γ v e1 e2 T,
     Γ ⊢t v ⋮v TBool ->
@@ -83,17 +83,58 @@ Inductive tm_has_type : context -> tm -> ty -> Prop :=
     Γ ⊢t e2 ⋮t T ->
     Γ ⊢t (tmatchb v e1 e2) ⋮t T
 with value_has_type : context -> value -> ty -> Prop :=
-| T_Const : forall Γ (c: constant), Γ ⊢t c ⋮v (ty_of_const c)
-| T_Op : forall Γ (op: biop), Γ ⊢t op ⋮v (ty_of_op op)
+| T_Const : forall Γ (c: constant), ok Γ -> Γ ⊢t c ⋮v (ty_of_const c)
+| T_Op : forall Γ (op: biop), ok Γ -> Γ ⊢t op ⋮v (ty_of_op op)
 | T_Var : forall Γ (x: atom) T,
+    ok Γ ->
     ctxfind Γ x = Some T -> Γ ⊢t x ⋮v T
 | T_Lam : forall Γ Tx T e (L: aset),
-    (forall (x: atom), x ∉ L -> (Γ ++ [(x, Tx)]) ⊢t e ⋮t T) ->
+    (forall (x: atom), x ∉ L -> (Γ ++ [(x, Tx)]) ⊢t e ^t^ x ⋮t T) ->
     Γ ⊢t vlam Tx e ⋮v Tx ⤍ T
 | T_Fix : forall Γ (Tx: base_ty) T e (L: aset),
-    (forall (f: atom), f ∉ L -> (Γ ++ [(f, Tx ⤍ T)]) ⊢t vlam Tx e ⋮v T) ->
+    (forall (f: atom), f ∉ L -> (Γ ++ [(f, Tx ⤍ T)]) ⊢t (vlam Tx e) ^v^ f ⋮v (Tx ⤍ T)) ->
     Γ ⊢t vfix (Tx ⤍ T) (vlam Tx e) ⋮v Tx ⤍ T
 where "Γ '⊢t' t '⋮t' T" := (tm_has_type Γ t T) and "Γ '⊢t' t '⋮v' T" := (value_has_type Γ t T).
 
+Scheme value_has_type_mutual_rec := Induction for value_has_type Sort Prop
+    with tm_has_type_mutual_rec := Induction for tm_has_type Sort Prop.
+
 Global Hint Constructors tm_has_type: core.
 Global Hint Constructors value_has_type: core.
+
+Ltac instantiate_atom_listctx :=
+  let acc := collect_stales tt in
+  instantiate (1 := acc); intros; listctx_set_simpl;
+  repeat (match goal with
+          | [H: forall (x: atom), x ∉ ?L -> _, H': ?a ∉ _ ∪ (stale _) |- _ ] =>
+              assert (a ∉ L) as Htmp by fast_set_solver;
+              specialize (H a Htmp); clear Htmp; repeat destruct_hyp_conj; auto
+          end; simpl).
+
+Lemma basic_typing_regular_value: forall Γ v t, Γ ⊢t v ⋮v t -> ok Γ /\ lc v.
+Proof.
+  apply (value_has_type_mutual_rec
+           (fun Γ v t P => ok Γ /\ lc v)
+           (fun Γ e t P => ok Γ /\ lc e)
+        ); split; intros; repeat destruct_hyp_conj; auto;
+    try (match goal with
+         | [H: forall (x: atom), x ∉ ?L -> ok (?Γ ++ _) /\ lc ?e |- _ ] =>
+             specialize (H (fv_of_set L) (fv_of_set_fresh L));
+             destruct H; repeat destruct_hyp_conj
+         end; lc_solver; listctx_set_solver);
+  try (econstructor; auto; instantiate_atom_listctx).
+Qed.
+
+Lemma basic_typing_regular_tm: forall Γ e t, Γ ⊢t e ⋮t t -> ok Γ /\ lc e.
+Proof.
+  apply (tm_has_type_mutual_rec
+           (fun Γ v t P => ok Γ /\ lc v)
+           (fun Γ e t P => ok Γ /\ lc e)
+        ); split; intros; repeat destruct_hyp_conj; auto;
+    try (match goal with
+         | [H: forall (x: atom), x ∉ ?L -> ok (?Γ ++ _) /\ lc ?e |- _ ] =>
+             specialize (H (fv_of_set L) (fv_of_set_fresh L));
+             destruct H; repeat destruct_hyp_conj
+         end; lc_solver; listctx_set_solver);
+    try (econstructor; auto; instantiate_atom_listctx).
+Qed.
