new_proof/BasicTypingProp.v
@@ -1,0 +1,282 @@
+From stdpp Require Import mapset.
+From CT Require Import CoreLangProp.
+From CT Require Import ListCtx.
+From CT Require Import BasicTyping.
+From CT Require Import OperationalSemantics.
+
+
+Import Atom.
+Import CoreLang.
+Import Tactics.
+Import NamelessTactics.
+Import ListCtx.
+Import BasicTyping.
+Import OperationalSemantics.
+
+(* weakening *)
+
+Ltac sv :=
+  match goal with
+  | [H: ctxfind (?Γ1 ++ ?Γ3) ?x = Some ?T |- ctxfind (?Γ1 ++ ?Γ2 ++ ?Γ3) ?x = Some ?T ] =>
+      apply ctxfind_app_weaken; auto
+  end.
+
+Lemma basic_typing_weaken_value_aux: forall Γ (v: value) T,
+    Γ ⊢t v ⋮v T ->
+    (forall Γ1 Γ2 Γ3, Γ = Γ1 ++ Γ3 -> ok (Γ1 ++ Γ2 ++ Γ3) → (Γ1 ++ Γ2 ++ Γ3) ⊢t v ⋮v T).
+Proof.
+  apply (value_has_type_mutual_rec
+           (fun Γ v T P => ∀ (Γ1 Γ2 Γ3 : list (atom * ty)),
+                (Γ = Γ1 ++ Γ3) -> ok (Γ1 ++ Γ2 ++ Γ3) → (Γ1 ++ Γ2 ++ Γ3) ⊢t v ⋮v T)
+           (fun Γ e T P => ∀ (Γ1 Γ2 Γ3 : list (atom * ty)),
+                (Γ = Γ1 ++ Γ3) -> ok (Γ1 ++ Γ2 ++ Γ3) → (Γ1 ++ Γ2 ++ Γ3) ⊢t e ⋮t T)
+        ); simpl; intros; subst; econstructor; auto;
+    try (instantiate_atom_listctx; auto_apply; listctx_set_solver);
+    try listctx_set_solver.
+Qed.
+
+Lemma basic_typing_weaken_tm_aux: forall Γ (v: tm) T,
+    Γ ⊢t v ⋮t T ->
+    (forall Γ1 Γ2 Γ3, Γ = Γ1 ++ Γ3 -> ok (Γ1 ++ Γ2 ++ Γ3) → (Γ1 ++ Γ2 ++ Γ3) ⊢t v ⋮t T).
+Proof.
+  apply (tm_has_type_mutual_rec
+           (fun Γ v T P => ∀ (Γ1 Γ2 Γ3 : list (atom * ty)),
+                (Γ = Γ1 ++ Γ3) -> ok (Γ1 ++ Γ2 ++ Γ3) → (Γ1 ++ Γ2 ++ Γ3) ⊢t v ⋮v T)
+           (fun Γ e T P => ∀ (Γ1 Γ2 Γ3 : list (atom * ty)),
+                (Γ = Γ1 ++ Γ3) -> ok (Γ1 ++ Γ2 ++ Γ3) → (Γ1 ++ Γ2 ++ Γ3) ⊢t e ⋮t T)
+        ); simpl; intros; subst; econstructor; auto;
+    try (instantiate_atom_listctx; auto_apply; listctx_set_solver);
+    try listctx_set_solver.
+Qed.
+
+Lemma basic_typing_weaken_value: forall Γ1 Γ3 Γ2 (v: value) T,
+    (Γ1 ++ Γ3) ⊢t v ⋮v T -> ok (Γ1 ++ Γ2 ++ Γ3) -> (Γ1 ++ Γ2 ++ Γ3) ⊢t v ⋮v T.
+Proof.
+  intros. eapply basic_typing_weaken_value_aux; eauto.
+Qed.
+
+Lemma basic_typing_weaken_tm: forall Γ1 Γ3 Γ2 (v: tm) T,
+    (Γ1 ++ Γ3) ⊢t v ⋮t T -> ok (Γ1 ++ Γ2 ++ Γ3) -> (Γ1 ++ Γ2 ++ Γ3) ⊢t v ⋮t T.
+Proof.
+  intros. eapply basic_typing_weaken_tm_aux; eauto.
+Qed.
+
+Lemma basic_typing_weaken_value_pre: forall Γ1 Γ3 u T,
+    ok (Γ1 ++ Γ3) -> Γ1 ⊢t u ⋮v T -> (Γ1 ++ Γ3) ⊢t u ⋮v T.
+Proof.
+  intros. rewrite <- (app_nil_r Γ1) in H0. rewrite <- (app_nil_r (Γ1 ++ Γ3)).
+  rewrite <- app_assoc. apply basic_typing_weaken_value; auto. listctx_set_solver.
+Qed.
+
+Lemma basic_typing_weaken_tm_pre: forall Γ1 Γ3 u T,
+    ok (Γ1 ++ Γ3) -> Γ1 ⊢t u ⋮t T -> (Γ1 ++ Γ3) ⊢t u ⋮t T.
+Proof.
+  intros. rewrite <- (app_nil_r Γ1) in H0. rewrite <- (app_nil_r (Γ1 ++ Γ3)).
+  rewrite <- app_assoc. apply basic_typing_weaken_tm; auto. listctx_set_solver.
+Qed.
+
+Lemma basic_typing_weaken_value_post: forall Γ1 Γ3 u T,
+    ok (Γ1 ++ Γ3) -> Γ3 ⊢t u ⋮v T -> (Γ1 ++ Γ3) ⊢t u ⋮v T.
+Proof.
+  intros. rewrite <- (app_nil_l Γ3) in H0. rewrite <- (app_nil_l (Γ1 ++ Γ3)).
+  apply basic_typing_weaken_value; auto.
+Qed.
+
+Lemma basic_typing_weaken_tm_post: forall Γ1 Γ3 u T,
+    ok (Γ1 ++ Γ3) -> Γ3 ⊢t u ⋮t T -> (Γ1 ++ Γ3) ⊢t u ⋮t T.
+Proof.
+  intros. rewrite <- (app_nil_l Γ3) in H0. rewrite <- (app_nil_l (Γ1 ++ Γ3)).
+  apply basic_typing_weaken_tm; auto.
+Qed.
+
+(* subst *)
+
+Ltac basic_typing_solver1 :=
+  listctx_set_simpl;
+  (match goal with
+   | [H: ?Γ1 ⊢t ?u ⋮v ?T |- (?Γ1 ++ ?Γ2) ⊢t ?u ⋮v ?T ] =>
+       apply basic_typing_weaken_value_pre; auto; try listctx_set_solver
+   | [H: ctxfind _ ?x = Some ?T |- _ ⊢t (vfvar ?x) ⋮v ?T ] => constructor; listctx_set_solver
+   | [H: ?Γ2 ⊢t ?u ⋮v ?T |- (?Γ1 ++ ?Γ2) ⊢t ?u ⋮v ?T ] => apply basic_typing_weaken_value_post; auto; try listctx_set_solver
+   | [H: _ ⊢t ?u ⋮v _ |- lc (tvalue ?u)] => apply basic_typing_regular_value in H; destruct H; auto
+   | [H: _ ⊢t ?u ⋮t _ |- lc ?u] => apply basic_typing_regular_tm in H; destruct H; auto
+   end || lc_solver ||
+       listctx_set_solver).
+
+Lemma basic_typing_subst_value_aux: forall Γ (v: value) T,
+    Γ ⊢t v ⋮v T ->
+    (forall Γ1 z u U Γ3, Γ = Γ1 ++ [(z, U)] ++ Γ3 -> Γ1 ⊢t u ⋮v U -> (Γ1 ++ Γ3) ⊢t {z := u}v v ⋮v T).
+Proof.
+  apply (value_has_type_mutual_rec
+           (fun Γ v T P => forall Γ1 z u U Γ3,
+                Γ = Γ1 ++ [(z, U)] ++ Γ3 -> Γ1 ⊢t u ⋮v U -> (Γ1 ++ Γ3) ⊢t {z := u}v v ⋮v T)
+           (fun Γ e T P => forall Γ1 z u U Γ3,
+                Γ = Γ1 ++ [(z, U)] ++ Γ3 -> Γ1 ⊢t u ⋮v U -> (Γ1 ++ Γ3) ⊢t {z := u}t e ⋮t T)
+        ); simpl; intros; subst; listctx_set_simpl;
+    try (var_dec_solver; basic_typing_solver1);
+    try (econstructor; listctx_set_solver).
+  - econstructor. instantiate_atom_listctx.
+    rewrite <- subst_open_var_tm; basic_typing_solver1.
+  - econstructor. instantiate_atom_listctx.
+    rewrite <- subst_open_var_tm; basic_typing_solver1.
+  - econstructor. instantiate (1:= T1). basic_typing_solver1.
+    instantiate_atom_listctx; rewrite <- subst_open_var_tm; basic_typing_solver1.
+  - econstructor.
+    instantiate (1:= T1). basic_typing_solver1.
+    instantiate (1:= T2). basic_typing_solver1.
+    instantiate (1:= Tx). basic_typing_solver1.
+    instantiate_atom_listctx; rewrite <- subst_open_var_tm; basic_typing_solver1.
+  - econstructor.
+    instantiate (1:= Tx). instantiate (1:= T1). basic_typing_solver1. basic_typing_solver1.
+    instantiate_atom_listctx; rewrite <- subst_open_var_tm; basic_typing_solver1.
+Qed.
+
+Lemma basic_typing_subst_tm_aux: forall Γ (v: tm) T,
+    Γ ⊢t v ⋮t T ->
+    (forall Γ1 z u U Γ3, Γ = Γ1 ++ [(z, U)] ++ Γ3 -> Γ1 ⊢t u ⋮v U -> (Γ1 ++ Γ3) ⊢t {z := u}t v ⋮t T).
+Proof.
+  apply (tm_has_type_mutual_rec
+           (fun Γ v T P => forall Γ1 z u U Γ3,
+                Γ = Γ1 ++ [(z, U)] ++ Γ3 -> Γ1 ⊢t u ⋮v U -> (Γ1 ++ Γ3) ⊢t {z := u}v v ⋮v T)
+           (fun Γ e T P => forall Γ1 z u U Γ3,
+                Γ = Γ1 ++ [(z, U)] ++ Γ3 -> Γ1 ⊢t u ⋮v U -> (Γ1 ++ Γ3) ⊢t {z := u}t e ⋮t T)
+        ); simpl; intros; subst; listctx_set_simpl;
+    try (var_dec_solver; basic_typing_solver1);
+    try (econstructor; listctx_set_solver).
+  - econstructor. instantiate_atom_listctx.
+    rewrite <- subst_open_var_tm; basic_typing_solver1.
+  - econstructor. instantiate_atom_listctx.
+    rewrite <- subst_open_var_tm; basic_typing_solver1.
+  - econstructor. instantiate (1:= T1). basic_typing_solver1.
+    instantiate_atom_listctx; rewrite <- subst_open_var_tm; basic_typing_solver1.
+  - econstructor.
+    instantiate (1:= T1). basic_typing_solver1.
+    instantiate (1:= T2). basic_typing_solver1.
+    instantiate (1:= Tx). basic_typing_solver1.
+    instantiate_atom_listctx; rewrite <- subst_open_var_tm; basic_typing_solver1.
+  - econstructor.
+    instantiate (1:= Tx). instantiate (1:= T1). basic_typing_solver1. basic_typing_solver1.
+    instantiate_atom_listctx; rewrite <- subst_open_var_tm; basic_typing_solver1.
+Qed.
+
+Lemma basic_typing_subst_value: forall Γ1 z u U Γ3 (v: value) T,
+    (Γ1 ++ [(z, U)] ++ Γ3) ⊢t v ⋮v T -> Γ1 ⊢t u ⋮v U -> (Γ1 ++ Γ3) ⊢t {z := u}v v ⋮v T.
+Proof.
+  intros. eapply basic_typing_subst_value_aux; eauto.
+Qed.
+
+Lemma basic_typing_subst_tm: forall Γ1 z u U Γ3 (v: tm) T,
+    (Γ1 ++ [(z, U)] ++ Γ3) ⊢t v ⋮t T -> Γ1 ⊢t u ⋮v U -> (Γ1 ++ Γ3) ⊢t {z := u}t v ⋮t T.
+Proof.
+  intros. eapply basic_typing_subst_tm_aux; eauto.
+Qed.
+
+Lemma basic_typing_subst_value_pre: forall Γ1 z u U (v: value) T,
+    (Γ1 ++ [(z, U)]) ⊢t v ⋮v T -> Γ1 ⊢t u ⋮v U -> Γ1 ⊢t {z := u}v v ⋮v T.
+Proof.
+  intros. rewrite <- (app_nil_r (Γ1 ++ [(z, U)])) in H. rewrite <- app_assoc in H.
+  rewrite <- (app_nil_r Γ1).
+  eapply basic_typing_subst_value; eauto.
+Qed.
+
+Lemma basic_typing_subst_tm_pre: forall Γ1 z u U (v: tm) T,
+    (Γ1 ++ [(z, U)]) ⊢t v ⋮t T -> Γ1 ⊢t u ⋮v U -> Γ1 ⊢t {z := u}t v ⋮t T.
+Proof.
+  intros. rewrite <- (app_nil_r (Γ1 ++ [(z, U)])) in H. rewrite <- app_assoc in H.
+  rewrite <- (app_nil_r Γ1).
+  eapply basic_typing_subst_tm; eauto.
+Qed.
+
+(* Lemma basic_typing_subst_value_post *)
+
+Ltac basic_typing_simpl1 :=
+  listctx_set_simpl;
+  repeat match goal with
+  | [H: ?Γ ⊢t (tvalue ?v) ⋮t ?T |- _ ] => inversion H; subst; clear H; auto
+  end.
+
+
+Lemma eval_op_type_safe: forall op c1 c2 c3 (T1 T2 T3: base_ty),
+  eval_op op c1 c2 c3 ->
+  ty_of_op op = T1 ⤍ T2 ⤍ T3 ->
+  ty_of_const c1 = T1 /\ ty_of_const c2 = T2 /\ ty_of_const c3 = T3.
+Proof.
+  repeat split; intros; destruct op; inversion H; subst; rewrite op_ty_spec in H0; inversion H0; subst; auto.
+Qed.
+
+Lemma eval_op_preservation_aux: forall Γ op c1 c2 c3 (T1 T2 T3: base_ty),
+    eval_op op c1 c2 c3 ->
+    ty_of_op op = T1 ⤍ T2 ⤍ T3 ->
+    ok Γ ->
+    Γ ⊢t c1 ⋮v T1 /\ Γ ⊢t c2 ⋮v T2 /\ Γ ⊢t c3 ⋮v T3.
+Proof.
+  intros.
+  assert (ty_of_const c1 = T1 /\ ty_of_const c2 = T2 /\ ty_of_const c3 = T3) by (eapply eval_op_type_safe; eauto).
+  repeat destruct_hyp_conj; subst. repeat split; auto.
+Qed.
+
+Lemma eval_op_preservation: forall Γ op c1 c2 c3 (T1 T2 T3: base_ty),
+    eval_op op c1 c2 c3 ->
+    Γ ⊢t op ⋮v T1 ⤍ T2 ⤍ T3 ->
+    Γ ⊢t c1 ⋮v T1 /\ Γ ⊢t c2 ⋮v T2 /\ Γ ⊢t c3 ⋮v T3.
+Proof.
+  intros.
+  inversion H0; subst.
+  eapply eval_op_preservation_aux; eauto.
+Qed.
+
+Ltac basic_typing_solver2 :=
+  basic_typing_simpl1;
+  try match goal with
+      | [H: ?Γ ⊢t (vbiop _) ⋮v _ ⤍ _ ⤍ ?T |- ?Γ ⊢t (vconst _) ⋮v ?T ] => eapply eval_op_preservation; eauto
+      end;
+  basic_typing_solver1.
+
+Ltac auto_pose_fv a Ha :=
+  let acc := collect_stales tt in pose (fv_of_set acc) as a;
+                                  pose (fv_of_set_fresh acc) as Ha.
+
+Ltac perservation_aux a Ha Tx :=
+  match goal with
+  | [H: forall (x:atom), _ -> _ ⊢t ?e ^t^ (vfvar x) ⋮t ?T |- _ ⊢t ?e ^t^ ?v ⋮t ?T ] =>
+      auto_pose_fv a Ha; rewrite <- (subst_intro_tm _ a);
+      try (eapply basic_typing_subst_tm_pre; try basic_typing_solver2; apply H; basic_typing_solver2);
+      try (apply basic_typing_subst_tm_pre with (U := Tx); basic_typing_solver2);
+      try basic_typing_solver2
+  end.
+
+(* perservation *)
+Lemma preservation: forall Γ T (e e': tm), e ↪ e' -> Γ ⊢t e ⋮t T -> Γ ⊢t e' ⋮t T.
+Proof.
+  intros. generalize dependent e'.
+  induction H0; intros; auto;
+    match goal with
+    | [H: _ ↪ _ |- _ ] => inversion H; subst
+    end; auto.
+  - econstructor; auto; instantiate_atom_listctx; auto_apply; listctx_set_solver.
+  - perservation_aux a Ha Tx.
+  - perservation_aux a Ha Tx.
+  - inversion H; subst; clear H. econstructor. instantiate (1:= Tx).
+    + perservation_aux a Ha Tx.
+    + instantiate_atom_listctx; auto_apply; listctx_set_solver.
+  - inversion H; subst; clear H. auto_pose_fv a Ha. eapply T_LetApp with (T1:=T1) (Tx:=Tx); auto.
+    + rewrite <- (subst_intro_value _ a).
+      eapply basic_typing_subst_value_pre; try basic_typing_solver2. apply H6; basic_typing_solver2.
+      econstructor; basic_typing_solver2. basic_typing_solver2. basic_typing_solver2.
+    + instantiate_atom_listctx; auto_apply; listctx_set_solver.
+Qed.
+
+(* multi preservation *)
+
+Lemma multi_preservation: forall Γ T (e e': tm), e ↪* e' -> Γ ⊢t e ⋮t T -> Γ ⊢t e' ⋮t T.
+Proof.
+  intros.
+  induction H; auto.
+  - apply IHmultistep. eapply preservation; eauto.
+Qed.
+
+Lemma multi_preservation_value: forall Γ T (e: tm) (v: value), e ↪* v -> Γ ⊢t e ⋮t T -> Γ ⊢t v ⋮v T.
+Proof.
+  intros.
+  eapply multi_preservation in H0; eauto. inversion H0; subst; auto.
+Qed.
