new_proof/TermOrdering.v
@@ -1,0 +1,102 @@
+From stdpp Require Import mapset.
+From Coq Require Import Logic.ClassicalFacts.
+From Coq Require Import Classical.
+From CT Require Import CoreLang.
+From CT Require Import CoreLangProp.
+From CT Require Import OperationalSemantics.
+
+Import Atom.
+Import CoreLang.
+Import Tactics.
+Import NamelessTactics.
+Import OperationalSemantics.
+
+Definition termR: relation tm := fun (e e': tm) => forall (v: value), e ↪* v -> e' ↪* v.
+Notation " e1 '<-<' e2 " := (termR e1 e2) (at level 10).
+Notation " e1 '>=<' e2 " := (termR e1 e2 /\ termR e2 e1) (at level 10).
+
+#[global]
+Instance termR_refl: Reflexive termR.
+Proof. intros e v. auto. Qed.
+Arguments termR_refl /.
+
+#[global]
+Instance termR_trans: Transitive termR.
+Proof. intros e1 e2 e3. unfold termR. intros. auto. Qed.
+Arguments termR_trans /.
+
+Lemma tlete_terr_exfalso: forall e (v: value), ~ tlete terr e ↪* v.
+Proof.
+  intros. intro H.
+  inversion H; subst. inversion H0; subst. inversion H6.
+Qed.
+
+Lemma tlete_value_exists: forall e (v_x v: value), tlete v_x e ↪* v <-> lc v_x /\ body e /\ e ^t^ v_x ↪* v.
+Proof.
+  split; intros.
+  - inversion H; subst. inversion H0; subst; auto. inversion H6.
+  - econstructor; repeat destruct_hyp_conj; auto. instantiate (1:= e ^t^ v_x). constructor; auto.
+    auto.
+Qed.
+
+Ltac op_simpl :=
+  match goal with
+  | [H: tlete terr _ ↪* (tvalue _) |- _ ] => apply tlete_terr_exfalso in H; inversion H
+  | [H: tlete (tvalue _) _ ↪* (tvalue _) |- _ ] => rewrite tlete_value_exists in H; repeat destruct_hyp_conj; auto
+  | [ |- ex (fun v_x => tvalue ?v ↪* tvalue v_x /\ _)] => exists v; split; auto
+  end.
+
+Lemma let_reduction_spec_forward_one_step: forall (e_x: tm) e (e': tm),
+    tlete e_x e ↪ e' -> (exists (v_x: value), e_x = v_x /\ e' = e ^t^ v_x) \/ (exists (e_x': tm), e_x ↪ e_x' /\ e' = tlete e_x' e).
+Proof.
+  intros.
+  inversion H; subst; clear H.
+  - right. exists e1'. split; auto.
+  - left. exists v1. split; auto.
+Qed.
+
+(* Need logical relation *)
+
+Lemma let_reduction_spec_forward: forall (e_x: tm) e (v: value),
+    (tlete e_x e ↪* v -> exists (v_x: value), e_x ↪* v_x /\ e ^t^ v_x ↪* v).
+Proof.
+  induction e_x; induction e; intros; try op_simpl; try (op_simpl; eexists; split; eauto).
+  - admit.
+  - op_simpl.
+    
+    end.
+      exists v. split; auto.
+  - op_simpl.
+  - op_simpl. eexists. split; eauto.
+  - specialize (IHe_x1 e_x2)
+
+Lemma let_reduction_spec_forward: forall (e_x: tm) e (v: value),
+    (tlete e_x e ↪* v -> exists (v_x: value), e_x ↪* v_x /\ e ^t^ v_x ↪* v).
+Proof.
+  induction e_x; intros.
+  - op_simpl.
+  - op_simpl. exists v0. split; auto.
+  - 
+
+    
+
+    admit.
+  - 
+  intros.
+  induction H0. admit.
+
+Lemma let_reduction_spec_tm: forall (e_x: tm) e (v: value),
+    lc e_x ->
+    (tlete e_x e ↪* v <-> exists (v_x: value), e_x ↪* v_x /\ e ^t^ v_x ↪* v).
+Proof.
+
+
+(* Lemma termR_fst: forall (e e': tm), termR e e' -> (forall (v: value), e -->* v -> e' -->* v). *)
+(* Proof. intros. destruct H. auto. Qed. *)
+
+(* Global Hint Resolve termR_fst: core. *)
+
+(* Lemma termR_snd: forall (e e': tm), termR e e' -> (forall Gamma T, Gamma \N- e \Tin T -> Gamma \N- e' \Tin T). *)
+(* Proof. intros. destruct H. eapply H1. auto. Qed. *)
+
+(* Global Hint Resolve termR_snd: core. *)
